SimSystem compiles, working on others

compose/SimSystem.v
@@ -7,26 +7,78 @@ Require Import Smallstep Simulation.
 Require Import CoqlibC.
 
 Require Import Mod ModSem Skeleton System.
-Require Import SimMem Sound SimSymb Syntax.
+Require Import SimProg SimMod SimModSem.
+Require Import SimMem Sound SimSymb Preservation Sem Syntax.
 
 Set Implicit Arguments.
 
 
 Section SIM.
+
   Context `{SM: SimMem.class}.
   Context `{SU: Sound.class}.
   Context {SS: SimSymb.class SM}.
 
-  Variables p: program.
-  System.module p
-  Definition mp: ModPair.t := SimSymb.mk_mp (RTLC.module prog) (RTLC.module tprog).
+  Variables pp: ProgPair.t.
+  Hypothesis (SIMPROG: ProgPair.sim pp).
+  Let p_src: program := (ProgPair.src pp).
+  Let p_tgt: program := (ProgPair.tgt pp).
+  Variable ss_link: SimSymb.t.
+  Hypothesis (SIMSK: SimSymb.wf ss_link).
+  (* Hypothesis (SSLE: Forall (fun mp => SimSymb.le (ModPair.ss mp) ss_link) pp). *)
+  (* Hypothesis (SKSRC: link_sk p_src = Some (SimSymb.src ss_link)). *)
+  (* Hypothesis (SKTGT: link_sk p_tgt = Some (SimSymb.tgt ss_link)). *)
 
-  Theorem sim_mod: ModPair.sim mp.
+  Theorem sim_system: exists mp,
+      (<<SYSSRC: mp.(ModPair.src) = (System.module ss_link.(SimSymb.src))>>) /\
+      (<<SYSTGT: mp.(ModPair.tgt) = (System.module ss_link.(SimSymb.tgt))>>) /\
+      (<<SYSSIM: ModPair.sim mp>>)
+  .
   Proof.
-    econs; ss.
-    - r. eapply Sk.match_program_eq; eauto. ii. destruct f1; ss.
-      + clarify. right. esplits; eauto.
-      + clarify. left. esplits; eauto.
-    - ii. inv SIMSKENVLINK. eapply sim_modsem; eauto.
+    exploit SimSymb.system_wf; eauto. i; des.
+    eexists (ModPair.mk _ _ ss_sys). ss.
+    esplits; eauto.
+    econs; ss. ii. unfold ModPair.to_msp. ss.
+    exploit system_local_preservation; eauto. intro SYSSU; des.
+    econs; eauto; ss.
+    { instantiate (2:= Empty_set). ii; ss. }
+    ii. inv SIMSKENV. ss.
+    split; cycle 1.
+    { ii; des. inv SAFESRC. inv SIMARGS; ss. esplits; eauto. econs; eauto. }
+    ii. sguard in SAFESRC. des. inv INITTGT.
+    inv SIMARGS; ss. clarify.
+    esplits; eauto.
+    { refl. }
+    { econs; eauto. }
+    pfold.
+    econs; eauto.
+    i.
+    econs; ss; cycle 2.
+    { eapply System.modsem_receptive; et. }
+    { u. esplits; ii; des; ss; eauto. inv H. }
+    ii. inv STEPSRC.
+    exploit SimSymb.system_axiom; eauto; swap 1 3; swap 2 4.
+    { econs; eauto. }
+    { ss. instantiate (1:= Retv.mk _ _). ss. eauto. }
+    { ss. }
+    { ss. }
+    i; des.
+    hexpl SimSymb.sim_skenv_func_bisim SIMGE0.
+    inv SIMGE0. exploit FUNCFSIM; eauto. i; des. clarify.
+    esplits; eauto.
+    { left. apply plus_one. econs.
+      - eapply System.modsem_determinate; et.
+      - ss. econs; eauto. }
+    left. pfold.
+    econs 4.
+    { refl. }
+    { eauto. }
+    { econs; eauto. }
+    { econs; eauto. }
+    { inv RETV; ss. unfold Retv.mk in *. clarify. econs; ss; eauto. }
+  Unshelve.
+    all: ss.
+    all: try eapply Ord.idx_bot; eauto.
   Qed.
+
 End SIM.
